Renaming, replace old solver with new one, hide rbt_assn and rbt_assn_cplx simp rule that unfolds the Branch by default

LLVM_DS_RBT/Setup.thy
@@ -1,631 +1,1 @@
-theory Setup
-  imports
-    Isabelle_LLVM.LLVM_DS_All
-    Abstract_Rbt
-    "Separation_Logic_Solver/Methods"
-begin
-
-
-subsection \<open>RBT NODE Datatype\<close>
-
-text_raw \<open>\snip{rbtnodedef}{1}{2}{%\<close>
-datatype ('key :: llvm_rep, 'value :: llvm_rep) rbt_node =
-  RBT_NODE
-  (color: "8 word")
-  (left: "('key,'value) rbt_node ptr")
-  (key: 'key) 
-  (val: 'value)
-  (right: "('key,'value) rbt_node ptr")
-text_raw \<open>}%endsnip\<close>
-
-hide_const (open) color left key val right
-
-
-type_synonym ('k, 'v) rbti = "('k, 'v) rbt_node ptr"  
-
-
-subsubsection \<open>Encoding to heap-representable\<close>
-   
-
-instantiation rbt_node :: (llvm_rep, llvm_rep) llvm_rep
-begin
-
-
-fun to_val_rbt_node where
-  "to_val_rbt_node (RBT_NODE col l_child k v r_child) = 
-    LL_STRUCT [to_val col, to_val l_child, to_val k, to_val v, to_val r_child]"
-
-
-fun from_val_rbt_node where
-  "from_val_rbt_node (LL_STRUCT [col, l_child_rep, k_rep, v_rep, r_child_rep]) = 
-    RBT_NODE (from_val col)
-             (from_val l_child_rep)
-             (from_val k_rep)
-             (from_val v_rep)
-             (from_val r_child_rep)"
-| "from_val_rbt_node _ = undefined"
-
-
-definition "struct_of_rbt_node (_::('a, 'b) rbt_node itself) =
-    VS_STRUCT [VS_INT 8, VS_PTR, struct_of TYPE('a), struct_of TYPE('b), VS_PTR]"
-
-
-definition "init_rbt_node \<equiv> RBT_NODE init init init init init"
-
-
-instance
-proof(standard, goal_cases)
-  case 1
-  then show ?case unfolding comp_def id_def 
-  proof
-    fix x:: "('a,'b) rbt_node"
-    show "from_val (to_val x) = x" by (cases x; simp)
-  qed
-next
-  case (2 v)
-  then show ?case
-    unfolding struct_of_rbt_node_def
-    by (cases v rule: from_val_rbt_node.cases; simp)
-next
-  case (3 x)
-  then show ?case
-    unfolding struct_of_rbt_node_def
-    by (cases x; simp)
-next
-  case 4
-  then show ?case
-    by (simp add: init_zero init_rbt_node_def struct_of_rbt_node_def to_val_word_def to_val_ptr_def null_def)
-qed
-end
-
-
-subsubsection \<open>Setup for LLVM code export\<close>
-text \<open>Declare structure to code generator.\<close>
-lemma to_val_rbt_node [ll_struct_of]:
-  "struct_of TYPE(('k::llvm_rep, 'v::llvm_rep) rbt_node) =
-      VS_STRUCT 
-      [
-        struct_of TYPE(8 word),
-        struct_of TYPE(('k, 'v) rbt_node ptr),
-        struct_of TYPE('k),
-        struct_of TYPE('v),
-        struct_of TYPE(('k, 'v) rbt_node ptr)
-      ]"
-  unfolding struct_of_rbt_node_def
-  by auto
-
-
-text \<open>Declare as named structure. Required b/c of circular reference.\<close>
-lemma [ll_identified_structures]:
-  "ll_is_identified_structure ''rbt_node'' TYPE((_, _) rbt_node)"  
-  unfolding ll_is_identified_structure_def
-    struct_of_rbt_node_def
-  by simp
-
-
-subsubsection \<open>Code Generator Preprocessor Setup\<close>  
-text \<open>The next two are auxiliary lemmas\<close>
-lemma rbt_node_insert_value [simp]:
-  "ll_insert_value (RBT_NODE c l k v r) ci 0 = Mreturn (RBT_NODE ci l k v r)"
-  "ll_insert_value (RBT_NODE c l k v r) li (Suc 0) = Mreturn (RBT_NODE c li k v r)"
-  "ll_insert_value (RBT_NODE c l k v r) ki 2 = Mreturn (RBT_NODE c l ki v r)"
-  "ll_insert_value (RBT_NODE c l k v r) vi 3 = Mreturn (RBT_NODE c l k vi r)"
-  "ll_insert_value (RBT_NODE c l k v r) ri 4 = Mreturn (RBT_NODE c l k v ri)"
-  by (simp_all add:
-      ll_insert_value_def llvm_insert_value_def
-      Let_def checked_from_val_def struct_of_rbt_node_def)
-
-
-lemma rbt_node_extract_value [simp]:
-  "ll_extract_value (RBT_NODE c l k v r) 0 = Mreturn c"
-  "ll_extract_value (RBT_NODE c l k v r) (Suc 0) = Mreturn l"
-  "ll_extract_value (RBT_NODE c l k v r) 2 = Mreturn k"
-  "ll_extract_value (RBT_NODE c l k v r) 3 = Mreturn v"
-  "ll_extract_value (RBT_NODE c l k v r) 4 = Mreturn r"
-  by (simp_all add:
-      ll_extract_value_def llvm_extract_value_def Let_def checked_from_val_def)
-
-
-text \<open>Lemmas to translate node construction and destruction\<close>
-lemma inline_return_node [llvm_pre_simp]: "Mreturn (RBT_NODE c l k v r) =
-   doM {
-    res \<leftarrow> ll_insert_value init c 0;
-    res \<leftarrow> ll_insert_value res l 1;
-    res \<leftarrow> ll_insert_value res k 2;
-    res \<leftarrow> ll_insert_value res v 3;
-    res \<leftarrow> ll_insert_value res r 4;
-    Mreturn res
-  }"
-  by (auto simp: init_rbt_node_def)
-
-
-lemma inline_node_case [llvm_pre_simp]: "
-  (case x of (RBT_NODE c l k v r) \<Rightarrow> f c l k v r) =
-   doM {
-    c \<leftarrow> ll_extract_value x 0;
-    l \<leftarrow> ll_extract_value x 1;
-    k \<leftarrow> ll_extract_value x 2;
-    v \<leftarrow> ll_extract_value x 3;
-    r \<leftarrow> ll_extract_value x 4;
-    f c l k v r
-  }"
-  apply (cases x)
-  by auto
-
-
-lemma inline_return_node_case [llvm_pre_simp]: 
-  "Mreturn (case x of (RBT_NODE c l k v r) \<Rightarrow> f c l k v r) = 
-  doM {
-    c \<leftarrow> ll_extract_value x 0;
-    l \<leftarrow> ll_extract_value x 1;
-    k \<leftarrow> ll_extract_value x 2;
-    v \<leftarrow> ll_extract_value x 3;
-    r \<leftarrow> ll_extract_value x 4;
-    Mreturn (f c l k v r)   
-  }"
-  apply (cases x)
-  by auto
-
-
-lemmas [llvm_inline] = 
-  rbt_node.color_def
-  rbt_node.left_def
-  rbt_node.key_def
-  rbt_node.val_def
-  rbt_node.right_def
-
-
-subsubsection \<open>Setters\<close>
-
-
-definition set_color :: 
-  "('k::llvm_rep, 'v::llvm_rep) rbt_node \<Rightarrow> 8 word \<Rightarrow> _"
-  where "set_color node col \<equiv> ll_insert_value node col 0"
-definition set_left :: 
-  "('k::llvm_rep, 'v::llvm_rep) rbt_node \<Rightarrow> ('k, 'v) rbti \<Rightarrow> _"
-  where "set_left node lhs \<equiv> ll_insert_value node lhs 1"
-definition set_key :: 
-  "('k::llvm_rep, 'v::llvm_rep) rbt_node \<Rightarrow> 'k \<Rightarrow> _"
-  where "set_key node k \<equiv> ll_insert_value node k 2"
-definition set_value :: 
-  "('k::llvm_rep, 'v::llvm_rep) rbt_node \<Rightarrow> 'v \<Rightarrow> _"
-  where "set_value node v \<equiv> ll_insert_value node v 3"
-definition set_right :: 
-  "('k::llvm_rep, 'v::llvm_rep) rbt_node \<Rightarrow> ('k, 'v) rbti \<Rightarrow> _"
-  where "set_right node rhs \<equiv> ll_insert_value node rhs 4"
-
-
-definition [llvm_pre_simp, simp]: 
-  "mod_ptr f n_p \<equiv>
-  doM {
-    n_pre \<leftarrow> ll_load n_p;
-    n_post \<leftarrow> f n_pre;
-    ll_store n_post n_p 
-  }"
-
-
-definition "set_color_p x \<equiv> mod_ptr (\<lambda>n. set_color n x)"
-definition "set_left_p x \<equiv> mod_ptr (\<lambda>n. set_left n x)"
-definition "set_key_p x \<equiv> mod_ptr (\<lambda>n. set_key n x)"
-definition "set_value_p x \<equiv> mod_ptr (\<lambda>n. set_value n x)"
-definition "set_right_p x \<equiv> mod_ptr (\<lambda>n. set_right n x)"
-
-
-lemmas [llvm_inline, simp] =
-  set_color_def
-  set_left_def
-  set_key_def
-  set_value_def
-  set_right_def
-
-  set_color_p_def
-  set_left_p_def
-  set_key_p_def
-  set_value_p_def
-  set_right_p_def
-
-
-subsection \<open>Color Assertion\<close>
-
-
-fun color_pred where 
-  "color_pred color.R rep = (rep = 0)"
-| "color_pred color.B rep = (rep = 1)"
-
-
-abbreviation "color_assn c ci \<equiv> \<up>(color_pred c ci)" 
-
-
-lemma color_assn_R_0 [fri_red_rules]:
-  "is_sep_red \<box> \<box> \<box> (color_assn color.R 0)"
-  apply (rule is_sep_redI)
-  apply isep_solver_keep
-  by simp_all
-
-
-lemma color_assn_B_1 [fri_red_rules]:
-  "is_sep_red \<box> \<box> \<box> (color_assn color.B 1)"
-  apply (rule is_sep_redI)
-  apply isep_solver_keep
-  by simp_all
-
-
-subsection \<open>Linorder Locale\<close>
-
-
-locale linorder_impl =
-  fixes 
-    abs_type :: "'a :: linorder itself" and
-    conc_type :: "'ai :: llvm_rep itself" and
-    lt_impl :: "'ai \<Rightarrow> 'ai \<Rightarrow> 1 word llM" and
-    elem_assn :: "('a, 'ai) dr_assn"
-  assumes lt_impl_rule [vcg_rules]: 
-    "llvm_htriple
-            (\<upharpoonleft>elem_assn lhs lhsi ** \<upharpoonleft>elem_assn rhs rhsi)
-            (lt_impl lhsi rhsi)
-            (\<lambda>r. 
-              \<upharpoonleft>bool.assn (lhs < rhs) r **
-              \<upharpoonleft>elem_assn lhs lhsi **
-              \<upharpoonleft>elem_assn rhs rhsi)"
-
-
-subsection \<open>RBT Locale\<close>
-
-
-locale monad_syntax_M_loc
-begin
-
-unbundle monad_syntax_M
-
-end
-
-
-locale rbt_impl_deps = 
-  monad_syntax_M_loc +
-  llvm_prim_ctrl_setup +
-  llvm_prim_arith_setup +
-  llvm_prim_setup
-
-
-locale rbt_impl =
-  linorder_impl key_type key_type_i lt_impl key_assn
-  for
-    key_type :: "'k :: linorder itself" and
-    key_type_i :: "'ki :: llvm_rep itself" and
-    value_type :: "'v itself" and
-    value_type_i :: "'vi :: llvm_rep itself" and    
-    
-    lt_impl and
-    key_assn and
-    key_delete :: "'ki \<Rightarrow> unit llM" and
-    value_assn :: "('v, 'vi) dr_assn" and
-    value_delete :: "'vi \<Rightarrow> unit llM" +
-  assumes
-    key_delete_rule [vcg_rules]: 
-    "
-      llvm_htriple
-      (\<upharpoonleft>key_assn k ki)
-      (key_delete ki)
-      (\<lambda>_. \<box>)
-    " and
-    value_delete_rule [vcg_rules]:
-    "
-      llvm_htriple
-      (\<upharpoonleft>value_assn v vi)
-      (value_delete vi)
-      (\<lambda>_. \<box>)
-    "
-begin
-interpretation rbt_impl_deps .
-
-
-subsection \<open>RBT Assertion\<close>
-  
-
-fun rbt_assn_cplx where
-  "rbt_assn_cplx rbt.Empty ptrs ex p = \<up>(p = null)"
-| "rbt_assn_cplx (rbt.Branch col lhs k v rhs) ptrs ex p =
-  (
-    EXS coli lhsi ki vi rhsi. 
-      \<up>(ptrs k = Some (p, vi)) **
-      \<upharpoonleft>ll_bpto (RBT_NODE coli lhsi ki vi rhsi) p **
-      color_assn col coli **
-      rbt_assn_cplx lhs ptrs ex lhsi **
-      \<upharpoonleft>key_assn k ki **
-      (if k \<in> ex then \<box> else \<upharpoonleft>value_assn v vi) **
-      rbt_assn_cplx rhs ptrs ex rhsi
-  )
-  "
-
-
-fun rbt_assn_cplx_full where "rbt_assn_cplx_full t ptrs ex ti = (rbt_assn_cplx t ptrs ex ti ** \<up>(is_rbt t))"
-
-
-fun rbt_assn :: "
-  ('k, 'v) rbt \<Rightarrow>
-  ('ki, 'vi) rbti \<Rightarrow>
-  ll_assn
-" where
-  "rbt_assn rbt.Empty p = \<up>(p=null)"
-| "rbt_assn (rbt.Branch col lhs k v rhs) p = (
-    EXS coli lhsi ki vi rhsi. 
-      \<upharpoonleft>ll_bpto (RBT_NODE coli lhsi ki vi rhsi) p **
-      color_assn col coli **
-      rbt_assn lhs lhsi **
-      \<upharpoonleft>key_assn k ki **
-      \<upharpoonleft>value_assn v vi **
-      rbt_assn rhs rhsi
-  )"
-
-
-fun rbt_assn_full where "rbt_assn_full t ti = (rbt_assn t ti ** \<up>(is_rbt t))"
-
-
-lemma rbt_assn_cplx_entails_rbt_assn:
-  "rbt_assn_cplx t ptrs {} ti \<turnstile> rbt_assn t ti"
-  apply (induction t arbitrary: ti)
-   apply simp
-  subgoal premises prems
-    apply simp
-    apply isep_elim_ex
-    apply (isep_solver_keep isep_intro: prems)
-    done
-  done
-
-
-lemma rbt_assn_cpxl_full_entails_rbt_assn_full:
-  "rbt_assn_cplx_full t ptrs {} ti \<turnstile> rbt_assn_full t ti"
-  apply simp
-  apply (isep_solver_keep isep_dest: rbt_assn_cplx_entails_rbt_assn)
-  apply simp
-  done
-
-
-lemma ptrs_upd_rbt_assn_cplx_sepI:
-  "kn \<notin> set(RBT_Impl.keys t) \<Longrightarrow>
-   rbt_assn_cplx t ptrs ex ti \<turnstile> rbt_assn_cplx t (\<lambda>x. if x = kn then p else ptrs x) ex ti"
-proof (induction t arbitrary: ti p)
-  case Empty show ?case by simp
-next
-  case (Branch c l k v r)
-  from Branch(3) show ?case
-    apply (auto split del: if_split) (*don't split if, it matches exactly*)
-    apply isep_solver_keep
-    apply isep_intro_ex
-    apply (isep_solver_keep isep_intro: Branch(1-2))
-    by simp_all
-qed
-
-
-lemma
-  ptrs_add_left_rbt_assn_cplx_sepI:
-  "dom ptrs2 \<inter> set (RBT_Impl.keys t) = {} \<Longrightarrow>
-  rbt_assn_cplx t ptrs1 ex ti \<turnstile> rbt_assn_cplx t (ptrs1 ++ ptrs2) ex ti"
-  proof (induction t arbitrary: ti)
-    case Empty
-    then show ?case by simp
-  next
-    case (Branch c l k v r)
-
-    from Branch(3) have l_int: "dom ptrs2 \<inter> set (RBT_Impl.keys l) = {}" by auto
-    from Branch(3) have r_int: "dom ptrs2 \<inter> set (RBT_Impl.keys r) = {}" by auto
-
-
-    note IH_l = Branch(1)[OF l_int]
-    note IH_r = Branch(2)[OF r_int]
-
-    show ?case
-      apply (simp split del: if_split)
-      apply isep_solver_keep
-      apply isep_intro_ex
-      apply (isep_solver_keep isep_dest: IH_l IH_r)
-      using Branch(3) by simp
-qed
-
-
-lemma ptrs_add_right_rbt_assn_cplx_sepI:
-  "dom ptrs1 \<inter> set (RBT_Impl.keys t) = {} \<Longrightarrow>
-  rbt_assn_cplx t ptrs2 ex ti \<turnstile> rbt_assn_cplx t (ptrs1 ++ ptrs2) ex ti"
-proof (induction t arbitrary: ti)
-  case Empty
-  then show ?case by simp
-next
-  case (Branch c l k v r)
-
-  from Branch(3) have l_int: "dom ptrs1 \<inter> set (RBT_Impl.keys l) = {}" by auto
-  from Branch(3) have r_int: "dom ptrs1 \<inter> set (RBT_Impl.keys r) = {}" by auto
-
-
-  note IH_l = Branch(1)[OF l_int]
-  note IH_r = Branch(2)[OF r_int]
-
-  show ?case
-    apply (simp split del: if_split)
-    apply isep_solver_keep
-     apply isep_intro_ex
-     apply (isep_solver_keep isep_dest: IH_l IH_r)
-    using Branch(3) by simp
-qed
-
-
-lemma rbt_sorted_key_uniqI:
-  "rbt_sorted (Branch c l k v r) \<Longrightarrow> k \<notin> set (RBT_Impl.keys l)"
-  "rbt_sorted (Branch c l k v r) \<Longrightarrow> k \<notin> set (RBT_Impl.keys r)"
-  apply simp_all
-  unfolding rbt_less_prop rbt_greater_prop
-  by blast+
-
-
-lemma rbt_sorted_subtrees_disjoint:
-  "rbt_sorted (Branch c l k v r) \<Longrightarrow> set (RBT_Impl.keys l) \<inter> set (RBT_Impl.keys r) = {}"
-  apply simp
-  unfolding rbt_less_prop rbt_greater_prop
-  by fastforce
-
-
-lemma rbt_assn_entails_rbt_assn_cplx:
-  "rbt_sorted t \<Longrightarrow> rbt_assn t ti \<turnstile> (EXS ptrs. rbt_assn_cplx t ptrs {} ti ** \<up>(dom ptrs = set (RBT_Impl.keys t)))"
-proof(induction t arbitrary: ti)
-  case Empty
-  then show ?case
-    apply simp
-    apply isep_intro_ex
-    apply isep_solver
-    apply simp
-    done
-next
-  case (Branch c l k v r)
-
-  show ?case
-    apply simp
-    apply (isep_solver_keep isep_dest: Branch(1-2))
-      apply simp
-    subgoal for x xa xb xc xd ptrs1 ptrs2
-      apply (isep_intro_ex_with "(ptrs1 ++ ptrs2)(k \<mapsto> (ti, ?x))")
-      apply simp
-      apply isep_intro_ex
-      apply (simp add: fun_upd_def)
-      apply (isep_solver isep_intro:
-          ptrs_upd_rbt_assn_cplx_sepI
-          ptrs_add_left_rbt_assn_cplx_sepI
-          ptrs_add_right_rbt_assn_cplx_sepI)
-            apply auto
-         apply (meson Branch.prems rbt_sorted_key_uniqI(1))
-        apply (meson Branch.prems rbt_sorted_key_uniqI(2))
-      using rbt_sorted_subtrees_disjoint Branch(3) apply fast+
-      done
-    using Branch(3) apply auto
-    done
-qed
-
-
-lemma [simp]: "rbt_assn t null = \<up>(t=rbt.Empty)"
-  by (cases t; simp add: pure_true_conv)
-
-
-lemma [simp]: "rbt_assn_full t null = \<up>(t=rbt.Empty)"
-  by (cases t; simp add: pure_true_conv)
-
-
-lemma [simp]: "rbt_assn_cplx t ptrs ex null = \<up>(t=rbt.Empty)"
-  by (cases t; simp add: pure_true_conv)
-
-
-subsection \<open>RBT Load Rule\<close>
-
-
-lemma load_rbt [vcg_rules]:
-  "
-    llvm_htriple
-    (rbt_assn (Branch col lhs k v rhs) ti)
-    (ll_load ti)
-    (\<lambda>r.
-      EXS coli lhsi ki vi rhsi.
-        \<upharpoonleft>ll_bpto (RBT_NODE coli lhsi ki vi rhsi) ti **
-        color_assn col coli **
-        rbt_assn lhs lhsi **
-        \<upharpoonleft>key_assn k ki **
-        \<upharpoonleft>value_assn v vi **  
-        rbt_assn rhs rhsi **
-        \<up>(r = RBT_NODE coli lhsi ki vi rhsi)
-    )
-  "
-  by vcg
-
-
-lemma load_rbt_cplx [vcg_rules]:
-  "
-    llvm_htriple
-    (rbt_assn_cplx (Branch col lhs k v rhs) ptrs ex ti)
-    (ll_load ti)
-    (\<lambda>r.
-      EXS coli lhsi ki vi rhsi.
-        \<up>(ptrs k = Some (ti, vi)) **
-        \<upharpoonleft>ll_bpto (RBT_NODE coli lhsi ki vi rhsi) ti **
-        color_assn col coli **
-        rbt_assn_cplx lhs ptrs ex lhsi **
-        \<upharpoonleft>key_assn k ki **
-        (if k \<in> ex then \<box> else \<upharpoonleft>value_assn v vi) **  
-        rbt_assn_cplx rhs ptrs ex rhsi **
-        \<up>(r = RBT_NODE coli lhsi ki vi rhsi)
-    )
-  "
-  unfolding rbt_assn_cplx.simps
-  by vcg
-
-
-subsection "Empty Function"
-
-
-definition empty :: "('ki, 'vi) rbti llM"
-  where [llvm_code]: "empty \<equiv> Mreturn null"
-
-
-lemma empty_correct [vcg_rules]: 
-  "llvm_htriple
-   \<box>
-   empty
-   (\<lambda> r. rbt_assn rbt.Empty r)"
-  unfolding empty_def
-  by vcg
-
-
-subsection "Reduction Rules"
-
-
-lemma unfold_rbt_assn_red_rule [fri_red_rules]: 
-  "
-    is_sep_red
-    \<box>
-    (color_assn c ci ** rbt_assn l li \<and>* \<upharpoonleft>key_assn k ki \<and>* \<upharpoonleft>value_assn v vi \<and>* rbt_assn r ri)
-    (\<upharpoonleft>ll_bpto (RBT_NODE ci li ki vi ri) ti)
-    (rbt_assn (rbt.Branch c l k v r) ti)
-  "
-  apply (rule is_sep_redI)
-  apply simp
-  subgoal premises prems for Ps Qs
-    apply (isep_solver isep_dest: prems)
-    (*
-    apply (sep_drule prems)
-    apply (simp only: fri_extract_simps entails_lift_extract_simps cong: entails_pre_cong)
-    apply clarify
-    apply fri
-    *)
-    done
-  done
-
-
-lemma unfold_rbt_assn_cplx_red_rule [fri_red_rules]: 
-  "
-    is_sep_red
-    \<box>
-    (
-      \<up>(ptrs k = Some (ti, vi)) **
-      color_assn c ci **
-      rbt_assn_cplx l ptrs ex li **
-      \<upharpoonleft>key_assn k ki **
-      (if k \<in> ex then \<box> else \<upharpoonleft>value_assn v vi) **
-      rbt_assn_cplx r ptrs ex ri
-    )
-    (\<upharpoonleft>ll_bpto (RBT_NODE ci li ki vi ri) ti)
-    (rbt_assn_cplx (rbt.Branch c l k v r) ptrs ex ti)
-  "
-  apply (rule is_sep_redI)
-  subgoal premises prems
-    apply (isep_drule drule: prems)
-    unfolding rbt_assn_cplx.simps
-    apply isep_solver_keep
-    done
-  done
-
-
-section \<open>Pure Part Simps\<close>
-
-
-lemmas pure_part_simps = pure_part_split_conj
-
-
-end
-
-
-end
+theory Setup  imports    Isabelle_LLVM.LLVM_DS_All    Abstract_Rbt    "Separation_Logic_Solver/Methods"beginsubsection \<open>RBT NODE Datatype\<close>text_raw \<open>\snip{rbtnodedef}{1}{2}{%\<close>datatype ('key :: llvm_rep, 'value :: llvm_rep) rbt_node =  RBT_NODE  (color: "8 word")  (left: "('key,'value) rbt_node ptr")  (key: 'key)   (val: 'value)  (right: "('key,'value) rbt_node ptr")text_raw \<open>}%endsnip\<close>hide_const (open) color left key val righttype_synonym ('k, 'v) rbti = "('k, 'v) rbt_node ptr"  subsubsection \<open>Encoding to heap-representable\<close>   instantiation rbt_node :: (llvm_rep, llvm_rep) llvm_repbeginfun to_val_rbt_node where  "to_val_rbt_node (RBT_NODE col l_child k v r_child) =     LL_STRUCT [to_val col, to_val l_child, to_val k, to_val v, to_val r_child]"fun from_val_rbt_node where  "from_val_rbt_node (LL_STRUCT [col, l_child_rep, k_rep, v_rep, r_child_rep]) =     RBT_NODE (from_val col)             (from_val l_child_rep)             (from_val k_rep)             (from_val v_rep)             (from_val r_child_rep)"| "from_val_rbt_node _ = undefined"definition "struct_of_rbt_node (_::('a, 'b) rbt_node itself) =    VS_STRUCT [VS_INT 8, VS_PTR, struct_of TYPE('a), struct_of TYPE('b), VS_PTR]"definition "init_rbt_node \<equiv> RBT_NODE init init init init init"instanceproof(standard, goal_cases)  case 1  then show ?case unfolding comp_def id_def   proof    fix x:: "('a,'b) rbt_node"    show "from_val (to_val x) = x" by (cases x; simp)  qednext  case (2 v)  then show ?case    unfolding struct_of_rbt_node_def    by (cases v rule: from_val_rbt_node.cases; simp)next  case (3 x)  then show ?case    unfolding struct_of_rbt_node_def    by (cases x; simp)next  case 4  then show ?case    by (simp add: init_zero init_rbt_node_def struct_of_rbt_node_def to_val_word_def to_val_ptr_def null_def)qedendsubsubsection \<open>Setup for LLVM code export\<close>text \<open>Declare structure to code generator.\<close>lemma to_val_rbt_node [ll_struct_of]:  "struct_of TYPE(('k::llvm_rep, 'v::llvm_rep) rbt_node) =      VS_STRUCT       [        struct_of TYPE(8 word),        struct_of TYPE(('k, 'v) rbt_node ptr),        struct_of TYPE('k),        struct_of TYPE('v),        struct_of TYPE(('k, 'v) rbt_node ptr)      ]"  unfolding struct_of_rbt_node_def  by autotext \<open>Declare as named structure. Required b/c of circular reference.\<close>lemma [ll_identified_structures]:  "ll_is_identified_structure ''rbt_node'' TYPE((_, _) rbt_node)"    unfolding ll_is_identified_structure_def    struct_of_rbt_node_def  by simpsubsubsection \<open>Code Generator Preprocessor Setup\<close>  text \<open>The next two are auxiliary lemmas\<close>lemma rbt_node_insert_value [simp]:  "ll_insert_value (RBT_NODE c l k v r) ci 0 = Mreturn (RBT_NODE ci l k v r)"  "ll_insert_value (RBT_NODE c l k v r) li (Suc 0) = Mreturn (RBT_NODE c li k v r)"  "ll_insert_value (RBT_NODE c l k v r) ki 2 = Mreturn (RBT_NODE c l ki v r)"  "ll_insert_value (RBT_NODE c l k v r) vi 3 = Mreturn (RBT_NODE c l k vi r)"  "ll_insert_value (RBT_NODE c l k v r) ri 4 = Mreturn (RBT_NODE c l k v ri)"  by (simp_all add:      ll_insert_value_def llvm_insert_value_def      Let_def checked_from_val_def struct_of_rbt_node_def)lemma rbt_node_extract_value [simp]:  "ll_extract_value (RBT_NODE c l k v r) 0 = Mreturn c"  "ll_extract_value (RBT_NODE c l k v r) (Suc 0) = Mreturn l"  "ll_extract_value (RBT_NODE c l k v r) 2 = Mreturn k"  "ll_extract_value (RBT_NODE c l k v r) 3 = Mreturn v"  "ll_extract_value (RBT_NODE c l k v r) 4 = Mreturn r"  by (simp_all add:      ll_extract_value_def llvm_extract_value_def Let_def checked_from_val_def)text \<open>Lemmas to translate node construction and destruction\<close>lemma inline_return_node [llvm_pre_simp]: "Mreturn (RBT_NODE c l k v r) =   doM {    res \<leftarrow> ll_insert_value init c 0;    res \<leftarrow> ll_insert_value res l 1;    res \<leftarrow> ll_insert_value res k 2;    res \<leftarrow> ll_insert_value res v 3;    res \<leftarrow> ll_insert_value res r 4;    Mreturn res  }"  by (auto simp: init_rbt_node_def)lemma inline_node_case [llvm_pre_simp]: "  (case x of (RBT_NODE c l k v r) \<Rightarrow> f c l k v r) =   doM {    c \<leftarrow> ll_extract_value x 0;    l \<leftarrow> ll_extract_value x 1;    k \<leftarrow> ll_extract_value x 2;    v \<leftarrow> ll_extract_value x 3;    r \<leftarrow> ll_extract_value x 4;    f c l k v r  }"  apply (cases x)  by autolemma inline_return_node_case [llvm_pre_simp]:   "Mreturn (case x of (RBT_NODE c l k v r) \<Rightarrow> f c l k v r) =   doM {    c \<leftarrow> ll_extract_value x 0;    l \<leftarrow> ll_extract_value x 1;    k \<leftarrow> ll_extract_value x 2;    v \<leftarrow> ll_extract_value x 3;    r \<leftarrow> ll_extract_value x 4;    Mreturn (f c l k v r)     }"  apply (cases x)  by autolemmas [llvm_inline] =   rbt_node.color_def  rbt_node.left_def  rbt_node.key_def  rbt_node.val_def  rbt_node.right_defsubsubsection \<open>Setters\<close>definition set_color ::   "('k::llvm_rep, 'v::llvm_rep) rbt_node \<Rightarrow> 8 word \<Rightarrow> _"  where "set_color node col \<equiv> ll_insert_value node col 0"definition set_left ::   "('k::llvm_rep, 'v::llvm_rep) rbt_node \<Rightarrow> ('k, 'v) rbti \<Rightarrow> _"  where "set_left node lhs \<equiv> ll_insert_value node lhs 1"definition set_key ::   "('k::llvm_rep, 'v::llvm_rep) rbt_node \<Rightarrow> 'k \<Rightarrow> _"  where "set_key node k \<equiv> ll_insert_value node k 2"definition set_value ::   "('k::llvm_rep, 'v::llvm_rep) rbt_node \<Rightarrow> 'v \<Rightarrow> _"  where "set_value node v \<equiv> ll_insert_value node v 3"definition set_right ::   "('k::llvm_rep, 'v::llvm_rep) rbt_node \<Rightarrow> ('k, 'v) rbti \<Rightarrow> _"  where "set_right node rhs \<equiv> ll_insert_value node rhs 4"definition [llvm_pre_simp, simp]:   "mod_ptr f n_p \<equiv>  doM {    n_pre \<leftarrow> ll_load n_p;    n_post \<leftarrow> f n_pre;    ll_store n_post n_p   }"definition "set_color_p x \<equiv> mod_ptr (\<lambda>n. set_color n x)"definition "set_left_p x \<equiv> mod_ptr (\<lambda>n. set_left n x)"definition "set_key_p x \<equiv> mod_ptr (\<lambda>n. set_key n x)"definition "set_value_p x \<equiv> mod_ptr (\<lambda>n. set_value n x)"definition "set_right_p x \<equiv> mod_ptr (\<lambda>n. set_right n x)"lemmas [llvm_inline, simp] =  set_color_def  set_left_def  set_key_def  set_value_def  set_right_def  set_color_p_def  set_left_p_def  set_key_p_def  set_value_p_def  set_right_p_defsubsection \<open>Color Assertion\<close>fun color_pred where   "color_pred color.R ci = (ci = 0)"| "color_pred color.B ci = (ci = 1)"abbreviation "color_assn c ci \<equiv> \<up>(color_pred c ci)" lemma color_assn_R_0 [fri_red_rules]:  "is_sep_red \<box> \<box> \<box> (color_assn color.R 0)"  apply (rule is_sep_redI)  apply sep  by simp_alllemma color_assn_B_1 [fri_red_rules]:  "is_sep_red \<box> \<box> \<box> (color_assn color.B 1)"  apply (rule is_sep_redI)  apply sep  by simp_allsubsection \<open>Linorder Locale\<close>locale linorder_impl =  fixes     abs_type :: "'a :: linorder itself" and    conc_type :: "'ai :: llvm_rep itself" and    lt_impl :: "'ai \<Rightarrow> 'ai \<Rightarrow> 1 word llM" and    elem_assn :: "('a, 'ai) dr_assn"  assumes lt_impl_rule [vcg_rules]:     "llvm_htriple            (\<upharpoonleft>elem_assn l li ** \<upharpoonleft>elem_assn r ri)            (lt_impl li ri)            (\<lambda>res.               \<upharpoonleft>bool.assn (l < r) res **              \<upharpoonleft>elem_assn l li **              \<upharpoonleft>elem_assn r ri)"subsection \<open>RBT Locale\<close>locale monad_syntax_M_locbeginunbundle monad_syntax_Mendlocale rbt_impl_deps =   monad_syntax_M_loc +  llvm_prim_ctrl_setup +  llvm_prim_arith_setup +  llvm_prim_setuplocale rbt_impl =  linorder_impl key_type key_type_i lt_impl key_assn  for    key_type :: "'k :: linorder itself" and    key_type_i :: "'ki :: llvm_rep itself" and    value_type :: "'v itself" and    value_type_i :: "'vi :: llvm_rep itself" and            lt_impl and    key_assn and    key_delete :: "'ki \<Rightarrow> unit llM" and    value_assn :: "('v, 'vi) dr_assn" and    value_delete :: "'vi \<Rightarrow> unit llM" +  assumes    key_delete_rule [vcg_rules]:     "      llvm_htriple      (\<upharpoonleft>key_assn k ki)      (key_delete ki)      (\<lambda>_. \<box>)    " and    value_delete_rule [vcg_rules]:    "      llvm_htriple      (\<upharpoonleft>value_assn v vi)      (value_delete vi)      (\<lambda>_. \<box>)    "begininterpretation rbt_impl_deps .subsection \<open>RBT Assertion\<close>  fun rbt_assn_cplx where  "rbt_assn_cplx rbt.Empty ptrs ex p = \<up>(p = null)"| "rbt_assn_cplx (rbt.Branch col lhs k v rhs) ptrs ex p =  (    EXS coli lhsi ki vi rhsi.       \<up>(ptrs k = Some (p, vi)) **      \<upharpoonleft>ll_bpto (RBT_NODE coli lhsi ki vi rhsi) p **      color_assn col coli **      rbt_assn_cplx lhs ptrs ex lhsi **      \<upharpoonleft>key_assn k ki **      (if k \<in> ex then \<box> else \<upharpoonleft>value_assn v vi) **      rbt_assn_cplx rhs ptrs ex rhsi  )  "declare rbt_assn_cplx.simps(2)[simp del]lemmas rbt_assn_cplx_unfold = rbt_assn_cplx.simps(2)fun rbt_assn_cplx_full where "rbt_assn_cplx_full t ptrs ex ti = (rbt_assn_cplx t ptrs ex ti ** \<up>(is_rbt t))"fun rbt_assn :: "  ('k, 'v) rbt \<Rightarrow>  ('ki, 'vi) rbti \<Rightarrow>  ll_assn" where  "rbt_assn rbt.Empty p = \<up>(p=null)"| "rbt_assn (rbt.Branch c l k v r) p = (    EXS ci li ki vi ri.       \<upharpoonleft>ll_bpto (RBT_NODE ci li ki vi ri) p **      color_assn c ci **      rbt_assn l li **      \<upharpoonleft>key_assn k ki **      \<upharpoonleft>value_assn v vi **      rbt_assn r ri  )"declare rbt_assn.simps(2)[simp del]lemmas rbt_assn_unfold = rbt_assn.simps(2)fun rbt_assn_full where "rbt_assn_full t ti = (rbt_assn t ti ** \<up>(is_rbt t))"lemma rbt_assn_cplx_entails_rbt_assn:  "rbt_assn_cplx t ptrs {} ti \<turnstile> rbt_assn t ti"  apply (induction t arbitrary: ti)  subgoal by (simp add: rbt_assn_unfold rbt_assn_cplx_unfold)  subgoal premises prems    apply (simp add: rbt_assn_unfold rbt_assn_cplx_unfold)    apply (sepE isep_intro: prems)    done  donelemma rbt_assn_cpxl_full_entails_rbt_assn_full:  "rbt_assn_cplx_full t ptrs {} ti \<turnstile> rbt_assn_full t ti"  apply simp  apply (sepEwith simp isep_dest: rbt_assn_cplx_entails_rbt_assn)  donefind_theorems set RBT_Impl.keyslemma ptrs_upd_rbt_assn_cplx_sepI:  "kn \<notin> rbt_key_set t \<Longrightarrow>   rbt_assn_cplx t ptrs ex ti \<turnstile> rbt_assn_cplx t (\<lambda>x. if x = kn then p else ptrs x) ex ti"proof (induction t arbitrary: ti p)  case Empty show ?case by (simp add: rbt_assn_cplx_unfold)next  case (Branch c l k v r)  from Branch(3) show ?case    apply (auto simp add: rbt_assn_cplx_unfold split del: if_split) (*don't split if, it matches exactly*)    apply (sepEwith simp isep_intro: Branch(1-2))    doneqedlemma  ptrs_add_left_rbt_assn_cplx_sepI:  "dom ptrs2 \<inter> rbt_key_set t = {} \<Longrightarrow>  rbt_assn_cplx t ptrs1 ex ti \<turnstile> rbt_assn_cplx t (ptrs1 ++ ptrs2) ex ti"  proof (induction t arbitrary: ti)    case Empty    then show ?case by (simp add: rbt_assn_cplx_unfold)  next    case (Branch c l k v r)    from Branch(3) have l_int: "dom ptrs2 \<inter> set (RBT_Impl.keys l) = {}" by auto    from Branch(3) have r_int: "dom ptrs2 \<inter> set (RBT_Impl.keys r) = {}" by auto    note IH_l = Branch(1)[OF l_int]    note IH_r = Branch(2)[OF r_int]    show ?case      apply (simp add: rbt_assn_cplx_unfold split del: if_split)      apply (sepEwith ignore isep_dest: IH_l IH_r)      using Branch(3) by simpqedlemma ptrs_add_right_rbt_assn_cplx_sepI:  "dom ptrs1 \<inter> set (RBT_Impl.keys t) = {} \<Longrightarrow>  rbt_assn_cplx t ptrs2 ex ti \<turnstile> rbt_assn_cplx t (ptrs1 ++ ptrs2) ex ti"proof (induction t arbitrary: ti)  case Empty  then show ?case by (simp add: rbt_assn_cplx_unfold)next  case (Branch c l k v r)  from Branch(3) have l_int: "dom ptrs1 \<inter> set (RBT_Impl.keys l) = {}" by auto  from Branch(3) have r_int: "dom ptrs1 \<inter> set (RBT_Impl.keys r) = {}" by auto  note IH_l = Branch(1)[OF l_int]  note IH_r = Branch(2)[OF r_int]  show ?case    apply (simp add: rbt_assn_cplx_unfold split del: if_split)    apply (sepEwith ignore isep_dest: IH_l IH_r)    using Branch(3) by simpqedlemma rbt_sorted_key_uniqI:  "rbt_sorted (Branch c l k v r) \<Longrightarrow> k \<notin> set (RBT_Impl.keys l)"  "rbt_sorted (Branch c l k v r) \<Longrightarrow> k \<notin> set (RBT_Impl.keys r)"  apply simp_all  unfolding rbt_less_prop rbt_greater_prop  by blast+lemma rbt_sorted_subtrees_disjoint:  "rbt_sorted (Branch c l k v r) \<Longrightarrow> set (RBT_Impl.keys l) \<inter> set (RBT_Impl.keys r) = {}"  apply simp  unfolding rbt_less_prop rbt_greater_prop  by fastforcelemma rbt_assn_entails_rbt_assn_cplx:  "rbt_sorted t \<Longrightarrow> rbt_assn t ti \<turnstile> (EXS ptrs. rbt_assn_cplx t ptrs {} ti ** \<up>(dom ptrs = set (RBT_Impl.keys t)))"proof(induction t arbitrary: ti)  case Empty  then show ?case    apply -    apply (sepEwith simp)    apply (simp add: rbt_assn_unfold rbt_assn_cplx_unfold)    donenext  case (Branch c l k v r)  show ?case    apply (simp add: rbt_assn_unfold rbt_assn_cplx_unfold)    apply (isep_solver_keep isep_dest: Branch(1-2))      apply simp    subgoal for x xa xb xc xd ptrs1 ptrs2      apply (isep_intro_ex_with "(ptrs1 ++ ptrs2)(k \<mapsto> (ti, ?x))")      apply simp      apply isep_intro_ex      apply (simp add: fun_upd_def)      apply (sepwith ignore          isep_intro:          ptrs_upd_rbt_assn_cplx_sepI          ptrs_add_left_rbt_assn_cplx_sepI          ptrs_add_right_rbt_assn_cplx_sepI          ; sep_solves)            apply auto         apply (meson Branch.prems rbt_sorted_key_uniqI(1))        apply (meson Branch.prems rbt_sorted_key_uniqI(2))      using rbt_sorted_subtrees_disjoint Branch(3) apply fast+      done    using Branch(3) apply auto    doneqedlemma [simp]: "rbt_assn t null = \<up>(t=rbt.Empty)"  by (cases t; simp add: rbt_assn_unfold pure_true_conv)lemma [simp]: "rbt_assn_full t null = \<up>(t=rbt.Empty)"  by (cases t; simp add: pure_true_conv)lemma [simp]: "rbt_assn_cplx t ptrs ex null = \<up>(t=rbt.Empty)"  by (cases t; simp add: rbt_assn_cplx_unfold pure_true_conv)subsection \<open>Load Rule\<close>lemma load_rbt [vcg_rules]:  "    llvm_htriple    (rbt_assn (Branch c l k v r) ti)    (ll_load ti)    (\<lambda>res.      EXS ci li ki vi ri.        \<upharpoonleft>ll_bpto res ti **        color_assn c ci **        rbt_assn l li **        \<upharpoonleft>key_assn k ki **        \<upharpoonleft>value_assn v vi **          rbt_assn r ri **        \<up>(res = RBT_NODE ci li ki vi ri)    )  "  unfolding rbt_assn_unfold  apply vcg  donelemma load_rbt_non_null:  "    ti \<noteq> null \<Longrightarrow>    llvm_htriple    (rbt_assn t ti)    (ll_load ti)    (\<lambda>res.      EXS ci li ki vi ri c l k v r.        \<upharpoonleft>ll_bpto res ti **        color_assn c ci **        rbt_assn l li **        \<upharpoonleft>key_assn k ki **        \<upharpoonleft>value_assn v vi **          rbt_assn r ri **        \<up>(res = RBT_NODE ci li ki vi ri) **        \<up>(t = rbt.Branch c l k v r))  "  apply vcg  apply (cases t)  subgoal by (simp add: rbt_assn_unfold) (*contradiction*)  subgoal by vcg  donelemma load_rbt_cplx [vcg_rules]:  "    llvm_htriple    (rbt_assn_cplx (Branch col lhs k v rhs) ptrs ex ti)    (ll_load ti)    (\<lambda>r.      EXS coli lhsi ki vi rhsi.        \<up>(ptrs k = Some (ti, vi)) **        \<upharpoonleft>ll_bpto (RBT_NODE coli lhsi ki vi rhsi) ti **        color_assn col coli **        rbt_assn_cplx lhs ptrs ex lhsi **        \<upharpoonleft>key_assn k ki **        (if k \<in> ex then \<box> else \<upharpoonleft>value_assn v vi) **          rbt_assn_cplx rhs ptrs ex rhsi **        \<up>(r = RBT_NODE coli lhsi ki vi rhsi)    )  "  unfolding rbt_assn_cplx_unfold  by vcgsubsection \<open>Reduction Rules\<close>lemma unfold_rbt_assn_red_rule [fri_red_rules]:   "    is_sep_red    \<box>    (color_assn c ci \<and>* rbt_assn l li \<and>* \<upharpoonleft>key_assn k ki \<and>* \<upharpoonleft>value_assn v vi \<and>* rbt_assn r ri)    (\<upharpoonleft>ll_bpto (RBT_NODE ci li ki vi ri) ti)    (rbt_assn (rbt.Branch c l k v r) ti)  "  apply (rule is_sep_redI)  apply (simp add: rbt_assn_unfold)  subgoal premises prems for Ps Qs    apply (sepE isep_dest: prems)    (*    apply (sep_drule prems)    apply (simp only: fri_extract_simps entails_lift_extract_simps cong: entails_pre_cong)    apply clarify    apply fri    *)    done  donelemma unfold_rbt_assn_cplx_red_rule [fri_red_rules]:   "    is_sep_red    \<box>    (      \<up>(ptrs k = Some (ti, vi)) **      color_assn c ci **      rbt_assn_cplx l ptrs ex li **      \<upharpoonleft>key_assn k ki **      (if k \<in> ex then \<box> else \<upharpoonleft>value_assn v vi) **      rbt_assn_cplx r ptrs ex ri    )    (\<upharpoonleft>ll_bpto (RBT_NODE ci li ki vi ri) ti)    (rbt_assn_cplx (rbt.Branch c l k v r) ptrs ex ti)  "  apply (rule is_sep_redI)  subgoal premises prems    apply (isep_drule drule: prems)    unfolding rbt_assn_cplx_unfold    apply sepE    done  donesubsection \<open>Empty Constructor\<close>definition empty :: "('ki, 'vi) rbti llM"  where [llvm_code]: "empty \<equiv> Mreturn null"lemma empty_correct [vcg_rules]:   "llvm_htriple   \<box>   empty   (\<lambda> r. rbt_assn rbt.Empty r)"  unfolding empty_def  by vcgendend
